lean/Main.lean
@@ -17,7 +17,7 @@ def runFlowAnalysis (s : Stmt) : LoweredExpr ⊕ String :=
     -- TODO: labels should identify the program point at which each value comes into existence, but
     -- the syntax doesn't yet carry enough information to do that, so every value currently has the
     -- version `ValueVersion.unspecified`.  Until that changes, a single label suffices.
-    let runResult ← elabStmtImpl (ℓ := Unit) s ⟨⟩ FlowModelImpl.empty
+    let runResult ← elabStmtImpl (ℓ := Unit) s ⟨⟩ AlgState.initial
     pure runResult.fst
   match loweredResult with
     | .ok m => .inl m
